make graph

Spacetalk/Compiler.lean
@@ -31,38 +31,39 @@ def Step.BinaryOp.compile : Step.BinaryOp α β γ → SimpleDataflow.Ops [α.to
   | .mul => .binaryOp .mul
 
 class IndexConverter {α : Type u} {n m : Nat} (xs : Vector α n) (ys : Vector α m) :=
+  newConsumer : Fin m
   conv : Fin n → Fin m
   conv_congr : ∀ {i}, xs.get i = ys.get (conv i)
   conv_lt : ∀ ⦃i j⦄, i < j → conv i < conv j
+  conv_gt_consumer : ∀ {i}, newConsumer < conv i
 
-class IndexConverterGtZero {α : Type u} {n m : Nat} (xs : Vector α n) (ys : Vector α m) extends IndexConverter xs ys :=
-  conv_gt_zero: ∀ {i}, (h_m : 0 < m) → ⟨0, h_m⟩ < conv i
+-- def appendIdConverter : IndexConverter xs (xs.append ys) :=
+--   let conv : Fin xs.length → Fin (xs.append ys).length := λ i ↦ ⟨i.val, by have := i.isLt; linarith⟩
+--   have conv_congr : ∀ {i}, xs.get i = (xs.append ys).get (conv i) := by
+--     intro i
+--     simp [conv]
+--     apply Vector.get_append_left.symm
+--   have conv_lt : ∀ ⦃i j⦄, i < j → conv i < conv j := by intro i j; simp [conv]
+--   ⟨conv, conv_congr, conv_lt⟩
 
-def appendIdConverter : IndexConverter xs (xs.append ys) :=
-  let conv : Fin xs.length → Fin (xs.append ys).length := λ i ↦ ⟨i.val, by have := i.isLt; linarith⟩
-  have conv_congr : ∀ {i}, xs.get i = (xs.append ys).get (conv i) := by
-    intro i
-    simp [conv]
-    apply Vector.get_append_left.symm
-  have conv_lt : ∀ ⦃i j⦄, i < j → conv i < conv j := by intro i j; simp [conv]
-  ⟨conv, conv_congr, conv_lt⟩
-
-def consConverter : IndexConverterGtZero xs (x ::ᵥ xs.append ys) :=
+-- Assume new consumer is appended to the front
+def consConverter : IndexConverter xs (x ::ᵥ xs.append ys) :=
   let conv : Fin xs.length → Fin (x ::ᵥ xs.append ys).length := λ i ↦ ⟨i.val + 1, by have := i.isLt; linarith⟩
   have conv_congr : ∀ {i}, xs.get i = (x ::ᵥ xs.append ys).get (conv i) := by
     intro i
     rw [←(x ::ᵥ xs.append ys).get_tail ⟨i, Nat.lt_add_right _ i.isLt⟩]
     exact Vector.get_append_left.symm
   have conv_lt : ∀ ⦃i j⦄, i < j → conv i < conv j := by simp [conv]
-  have conv_gt_zero: ∀ {i}, _ → 0 < conv i := by
+  have conv_gt_zero: ∀ {i}, 0 < conv i := by
     intro i
     simp [conv]
     apply Fin.mk_lt_mk.mpr
     rw [Nat.zero_mod]
     simp
-  .mk conv_gt_zero (toIndexConverter := ⟨conv, conv_congr, conv_lt⟩)
+  ⟨0, conv, conv_congr, conv_lt, conv_gt_zero⟩
 
-def consAppendConverter {xs : Vector α n} {ys : Vector α m} : IndexConverterGtZero ys (x ::ᵥ xs.append ys) :=
+-- Assume new consumer is appended to the front
+def consAppendConverter {xs : Vector α n} {ys : Vector α m} : IndexConverter ys (x ::ᵥ xs.append ys) :=
   let conv : Fin m → Fin (n + m + 1) := λ i ↦ ⟨i.val + n + 1, by have := i.isLt; linarith⟩
   have conv_congr : ∀ {i}, ys.get i = (x ::ᵥ xs.append ys).get (conv i) := by
     intro i
@@ -71,31 +72,33 @@ def consAppendConverter {xs : Vector α n} {ys : Vector α m} : IndexConverterGt
     simp
     exact Vector.get_append_right.symm
   have conv_lt : ∀ ⦃i j⦄, i < j → conv i < conv j := by simp [conv]
-  have conv_gt_zero: ∀ {i}, _ → 0 < conv i := by
+  have conv_gt_zero: ∀ {i}, 0 < conv i := by
     intro i
     simp [conv]
     apply Fin.mk_lt_mk.mpr
     rw [Nat.zero_mod]
     simp
-  .mk conv_gt_zero (toIndexConverter := ⟨conv, conv_congr, conv_lt⟩)
+  ⟨0, conv, conv_congr, conv_lt, conv_gt_zero⟩
 
-def appendConverter {xs : Vector α n} {ys : Vector α m} (h_n : 0 < n) : IndexConverterGtZero ys (xs.append ys) :=
+def appendConverter {xs : Vector α n} {ys : Vector α m} (newConsumer : Fin n) : IndexConverter ys (xs.append ys) :=
   let conv : Fin m → Fin (n + m) := λ i ↦ ⟨i.val + n, by have := i.isLt; linarith⟩
   have conv_congr : ∀ {i}, ys.get i = (xs.append ys).get (conv i) := by
     intro i
     exact Vector.get_append_right.symm
   have conv_lt : ∀ ⦃i j⦄, i < j → conv i < conv j := by simp [conv]
-  have conv_gt_zero: ∀ {i}, (h_m : 0 < n + m) → ⟨0, h_m⟩ < conv i := by
-    intro i h_m
-    simp [conv]
-    apply Or.intro_right
-    exact h_n
-  .mk conv_gt_zero (toIndexConverter := ⟨conv, conv_congr, conv_lt⟩)
+  let newConsumer' : Fin (n + m) := ⟨newConsumer.val, Nat.lt_add_right m newConsumer.isLt⟩
+  have conv_gt_consumer: ∀ {i}, newConsumer' < conv i := by
+    intro i
+    simp [conv, newConsumer']
+    have := newConsumer.isLt
+    linarith
+  ⟨newConsumer', conv, conv_congr, conv_lt, conv_gt_consumer⟩
 
 /-- Assume new consumer has index 0. -/
 def convertFifosOutput {inputs outputs : List SimpleDataflow.Ty} {numNodes : Nat} {nodes : SDFNodeList numNodes}
-  (h_len : 0 < numNodes) (a : SDFConv aInp α) (newConsumerPort : Member α.toSDF (nodes.get ⟨0, h_len⟩).inputs)
-  (idxConv : IndexConverterGtZero a.g.nodes nodes)
+  (h_len : 0 < numNodes) (a : SDFConv aInp α)
+  (idxConv : IndexConverter a.g.nodes nodes)
+  (newConsumerPort : Member α.toSDF (nodes.get idxConv.newConsumer).inputs)
   (memConv : {t : SimpleDataflow.Ty} → Member t a.g.inputs → Member t inputs)
   : List (FIFO inputs outputs nodes) :=
   a.g.fifos.attach.map (
@@ -124,10 +127,10 @@ def convertFifosOutput {inputs outputs : List SimpleDataflow.Ty} {numNodes : Nat
         let fifo : AdvancingFIFO nodes := {
           t := f.t,
           producer := newProducer,
-          consumer := ⟨0, h_len⟩,
+          consumer := idxConv.newConsumer,
           producerPort := idxConv.conv_congr ▸ f.producerPort,
           consumerPort := h_ty_eq ▸ newConsumerPort,
-          adv := idxConv.conv_gt_zero h_len,
+          adv := idxConv.conv_gt_consumer,
         }
         .advancing fifo
       | .advancing f =>
@@ -157,10 +160,10 @@ def convertFifosOutput {inputs outputs : List SimpleDataflow.Ty} {numNodes : Nat
 theorem convertFifos_no_output
   {a : SDFConv aInp α}
   {h_len : 0 < numNodes}
-  {newConsumerPort : Member α.toSDF (nodes.get ⟨0, h_len⟩).inputs}
-  {idxConv : IndexConverterGtZero a.g.nodes nodes}
+  {idxConv : IndexConverter a.g.nodes nodes}
+  {newConsumerPort : Member α.toSDF (nodes.get idxConv.newConsumer).inputs}
   {memConv : {t : SimpleDataflow.Ty} → Member t a.g.inputs → Member t inputs}
-  : FIFO.getOutputs (convertFifosOutput h_len a newConsumerPort idxConv memConv) (outputs := outputs) = [] := by
+  : FIFO.getOutputs (convertFifosOutput h_len a idxConv newConsumerPort memConv) (outputs := outputs) = [] := by
   simp [List.eq_nil_iff_forall_not_mem, List.mem_filterMap]
   intro _ fifo h_mem
   have h_map := List.mem_map.mp h_mem
@@ -191,8 +194,8 @@ def zipGraph (op : Step.BinaryOp α β γ) (a : SDFConv aInp α) (b : SDFConv bI
   let opNode : SDFNode := ⟨[α.toSDF, β.toSDF], outputs, [], []ₕ, op.compile⟩
   let nodes := opNode ::ᵥ (a.g.nodes.append b.g.nodes)
 
-  let aFifosConverted : List (FIFO inputs outputs nodes) := convertFifosOutput (Nat.zero_lt_succ _) a .head consConverter .append_left
-  let bFifosConverted : List (FIFO inputs outputs nodes) := convertFifosOutput (Nat.zero_lt_succ _) b (.tail .head) consAppendConverter .append_right
+  let aFifosConverted : List (FIFO inputs outputs nodes) := convertFifosOutput (Nat.zero_lt_succ _) a consConverter .head .append_left
+  let bFifosConverted : List (FIFO inputs outputs nodes) := convertFifosOutput (Nat.zero_lt_succ _) b consAppendConverter (.tail .head) .append_right
 
   let newOutputFifo : OutputFIFO outputs nodes := ⟨γ.toSDF, 0, .head, .head⟩
   let newFifos := .output newOutputFifo :: (aFifosConverted ++ bFifosConverted)
@@ -235,27 +238,69 @@ def mapGraph (op : Step.UnaryOp α β) (a : SDFConv inp α) : SDFConv inp β :=
   | .addConst c => zipGraph .add (constValueGraph c) a
   | .mulConst c => zipGraph .mul (constValueGraph c) a
 
+set_option maxHeartbeats 900000
 def reduceBlock {α β : Step.Ty}
-  (op : Step.BinaryOp α β α) (len : Nat) (init : α.denote) (bs : SDFConv inp β)
+  (op : Step.BinaryOp α β α) (len : Nat) (init : α.denote) (b : SDFConv inp β)
   : SDFConv inp α :=
-  -- Counter Logic
-  -- let ctrWidth := (Nat.log2 len) + 1
-  -- let ctrTy : Ty := BitVecTy ctrWidth
-  -- let constOne : SDFNode := ⟨[], [ctrTy], [], []ₕ, .const 1⟩
-  -- let constZero : SDFNode := ⟨[], [ctrTy], [], []ₕ, .const 0⟩
-  -- let ctrUpdate : SDFNode := ⟨[ctrTy, ctrTy], [ctrTy], [], []ₕ, .binaryOp .add⟩
-  -- let constLen : SDFNode := ⟨[], [ctrTy], [], []ₕ, .const len⟩
-  -- let ctrMod : SDFNode := ⟨[ctrTy, ctrTy], [ctrTy], [], []ₕ, .binaryOp .umod⟩
-  -- let ctrComp : SDFNode := ⟨[ctrTy, ctrTy], [BoolTy], [], []ₕ, .binaryOp .eq⟩
+  let ctrWidth := (Nat.log2 len) + 1
+  let ctrTy : SimpleDataflow.Ty := SimpleDataflow.BitVecTy ctrWidth
 
-  -- let redux : SDFNode := ⟨[α, β], [α], [], []ₕ, op.compile⟩
-  -- let someWrap : SDFNode := ⟨[α], [α.toOption], [], []ₕ, .unaryOp .some⟩
-  -- let constNone : SDFNode := ⟨[], [α.toOption], [], []ₕ, .const none⟩
+  let redux : SDFNode := ⟨[α.toSDF, β.toSDF], [α.toSDF], [], []ₕ, op.compile⟩
 
-  -- let outputMux : SDFNode := ⟨[BoolTy, α.toOption, α.toOption], [α.toOption], [], []ₕ, .mux⟩
-  -- let accMux : SDFNode := ⟨[BoolTy, α, α], [α], [], []ₕ, .mux⟩
+  let constZero : SDFNode := ⟨[], [ctrTy], [], []ₕ, .const (some 0)⟩
+  let constOne : SDFNode := ⟨[], [ctrTy], [], []ₕ, .const (some 1)⟩
+  let constLen : SDFNode := ⟨[], [ctrTy], [], []ₕ, .const (some len)⟩
+  let constInit : SDFNode := ⟨[], [α.toSDF], [], []ₕ, .const (some init)⟩
 
-  -- let nodes : SDFNodeList _ := ctrMod ::ᵥ constLen ::ᵥ ctrUpdate ::ᵥ constOne ::ᵥ .nil;
+  let ctrUpdate : SDFNode := ⟨[ctrTy, ctrTy], [ctrTy], [], []ₕ, .binaryOp .add⟩
+  let ctrMod : SDFNode := ⟨[ctrTy, ctrTy], [ctrTy], [], []ₕ, .binaryOp .umod⟩
+  let ctrComp : SDFNode := ⟨[ctrTy, ctrTy], [SimpleDataflow.BoolTy], [], []ₕ, .binaryOp .eq⟩
+
+  let outputGuard : SDFNode := ⟨[SimpleDataflow.BoolTy, α.toSDF], [α.toSDF], [], []ₕ, .guard⟩
+  let accMux : SDFNode := ⟨[SimpleDataflow.BoolTy, α.toSDF, α.toSDF], [α.toSDF], [], []ₕ, .mux⟩
+  let ctrMux : SDFNode := ⟨[SimpleDataflow.BoolTy, ctrTy, ctrTy], [ctrTy], [], []ₕ, .mux⟩
+
+  let newNodes : SDFNodeList 11 := (
+    outputGuard ::ᵥ accMux ::ᵥ redux ::ᵥ
+    ctrMux ::ᵥ ctrComp ::ᵥ ctrMod ::ᵥ ctrUpdate ::ᵥ
+    constLen ::ᵥ constOne ::ᵥ constZero ::ᵥ constInit ::ᵥ .nil
+  )
+  let nodes : SDFNodeList (11 + b.g.nodes.length) := newNodes.append b.g.nodes
+  have h_lt {i : Nat} (h : i < 11) : i < nodes.length := Nat.lt_add_right b.g.nodes.length h
+
+  let outputGuardIdx : Fin nodes.length := ⟨0, h_lt (by simp)⟩
+  let accMuxIdx : Fin nodes.length := ⟨1, h_lt (by simp)⟩
+  let reduxIdx : Fin nodes.length := ⟨2, h_lt (by simp)⟩
+  let ctrMuxIdx : Fin nodes.length := ⟨3, h_lt (by simp)⟩
+  let ctrCompIdx : Fin nodes.length := ⟨4, h_lt (by simp)⟩
+  let ctrModIdx : Fin nodes.length := ⟨5, h_lt (by simp)⟩
+  let ctrUpdateIdx : Fin nodes.length := ⟨6, h_lt (by simp)⟩
+  let constLenIdx : Fin nodes.length := ⟨7, h_lt (by simp)⟩
+  let constOneIdx : Fin nodes.length := ⟨8, h_lt (by simp)⟩
+  let constZeroIdx : Fin nodes.length := ⟨9, h_lt (by simp)⟩
+  let constInitIdx : Fin nodes.length := ⟨10, h_lt (by simp)⟩
+
+  let inputs := b.g.inputs
+  let outputs := [α.toSDF]
+
+  let bFifosConverted : List (FIFO inputs outputs nodes) := convertFifosOutput (by simp) b (appendConverter reduxIdx) (.tail .head) id
+
+  let newFifos : List (FIFO inputs outputs nodes) := [
+    .initialized ⟨α.toSDF, some init, accMuxIdx, reduxIdx, .head, .head⟩, -- accumulated value
+    .advancing ⟨α.toSDF, reduxIdx, accMuxIdx, .head, .tail .head, by simp [reduxIdx, accMuxIdx]⟩, -- redux output
+    .advancing ⟨α.toSDF, constInitIdx, accMuxIdx, .head, .tail (.tail .head), by simp [constInitIdx, accMuxIdx]⟩, -- redux initial value
+    .advancing ⟨SimpleDataflow.BoolTy, ctrCompIdx, accMuxIdx, .head, .head, by simp [ctrCompIdx, accMuxIdx]⟩, -- accum mux condition
+    .advancing ⟨SimpleDataflow.BoolTy, ctrCompIdx, outputGuardIdx, .head, .head, by simp [ctrCompIdx, outputGuardIdx]⟩,
+    .advancing ⟨α.toSDF, reduxIdx, outputGuardIdx, .head, .tail .head, by simp [reduxIdx, outputGuardIdx]⟩,
+    .output ⟨α.toSDF, outputGuardIdx, .head, .head⟩,
+
+    .initialized ⟨ctrTy, some 0, ctrModIdx, ctrUpdateIdx, .head, .head⟩, -- ctr + 1 - left arg
+    .advancing ⟨ctrTy, constOneIdx, ctrUpdateIdx, .head, .tail .head, by simp [constOneIdx, ctrUpdateIdx]⟩, -- ctr + 1 - right arg
+    .advancing ⟨ctrTy, ctrUpdateIdx, ctrModIdx, .head, .head, by simp [ctrUpdateIdx, ctrModIdx]⟩, -- ctr % len - left arg
+    .advancing ⟨ctrTy, constLenIdx, ctrModIdx, .head, .tail .head, by simp [constLenIdx, ctrModIdx]⟩, -- ctr % len - right arg
+    .advancing ⟨ctrTy, ctrModIdx, ctrCompIdx, .head, .head, by simp [ctrModIdx, ctrCompIdx]⟩, -- ctr == 0 - left arg
+    .advancing ⟨ctrTy, constZeroIdx, ctrCompIdx, .head, .tail .head, by simp [constZeroIdx, ctrCompIdx]⟩, -- ctr == 0 - right arg
+  ]
   sorry
 
 def Step.Prog.compile {inp : List Ty} {out : Ty} : Step.Prog inp out → SDFConv inp out
